ulib/experimental/Steel.Actions.fsti
@@ -70,7 +70,7 @@ val as_seq_lemma
 
 val index_array
   (#t:_)
-  (a:array_ref t)
+  (a:array_ref t{a =!= null_array t})
   (iseq: Ghost.erased (Seq.lseq t (U32.v (length a))))
   (p: permission{allows_read p})
   (i:U32.t{U32.v i < U32.v (length a)})
@@ -81,7 +81,7 @@ val index_array
 
 val upd_array
   (#t:_)
-  (a:array_ref t)
+  (a:array_ref t{a =!= null_array t})
   (iseq: Ghost.erased (Seq.lseq t (U32.v (length a))))
   (i:U32.t{U32.v i < U32.v (length a)})
   (v: t)
@@ -92,7 +92,7 @@ val upd_array
 
 val alloc_array
   (#t: _)
-  (len:U32.t{U32.v len > 0})
+  (len:U32.t)
   (init: t)
   : m_action
     emp
@@ -116,7 +116,7 @@ val share_array
     (pts_to_array a p iseq)
     (a':array_ref t{
       length a' = length a /\ offset a' = offset a /\ max_length a' = max_length a /\
-      address a = address a'
+      (a =!= null_array t ==> (a' =!= null_array t /\ address a = address a'))
     })
     (fun a' -> star
       (pts_to_array a (half_permission p) iseq)
@@ -128,7 +128,7 @@ val gather_array
   (a: array_ref t)
   (a':array_ref t{
     length a' = length a /\ offset a' = offset a /\ max_length a' = max_length a /\
-    address a = address a'
+    ((a =!= null_array t /\ a' =!= null_array t) ==> address a = address a')
   })
   (iseq: Ghost.erased (Seq.lseq t (U32.v (length a))))
   (p: permission{allows_read p})
@@ -146,15 +146,21 @@ val split_array
   (a: array_ref t)
   (iseq: Ghost.erased (Seq.lseq t (U32.v (length a))))
   (p: permission{allows_read p})
-  (i:U32.t{U32.v i > 0 /\ U32.v i < U32.v (length a)})
+  (i:U32.t{U32.v i < U32.v (length a)})
   : m_action
     (pts_to_array a p iseq)
-    (as:(array_ref t & array_ref t){(
-      length (fst as) = i /\ length (snd as) = U32.sub (length a) i /\
-      offset (fst as) = offset a /\ offset (snd as) = U32.add (offset a) i /\
-      max_length (fst as) = max_length a /\ max_length (snd as) = max_length a /\
-      address (fst as) = address a /\ address (snd as) = address a
-    )})
+    (as:(array_ref t & array_ref t){
+     length (fst as) = i /\ length (snd as) = U32.sub (length a) i /\
+      (a =!= null_array t ==>
+        (U32.v i > 0 ==> (fst as) =!= null_array t /\ offset (fst as) = offset a /\
+          address (fst as) = address a /\ max_length (fst as) = max_length a
+        ) /\
+        (U32.v i < U32.v (length a) ==> (snd as) =!= null_array t /\
+          offset (snd as) = U32.add (offset a) i /\
+          address (snd as) = address a /\ max_length (snd as) = max_length a
+        )
+      )
+    })
     (fun (a1, a2) -> star
       (pts_to_array a1 p (Seq.slice iseq 0 (U32.v i)))
       (pts_to_array a2 p (Seq.slice iseq (U32.v i) (U32.v (length a))))
@@ -164,7 +170,8 @@ val glue_array
   (#t: _)
   (a: array_ref t)
   (a': array_ref t{
-    address a = address a' /\ max_length a = max_length a' /\
+    ((a =!= null_array t /\ a' =!= null_array t) ==> address a = address a') /\
+    max_length a = max_length a' /\
     offset a' = U32.add (offset a) (length a)
   })
   (iseq: Ghost.erased (Seq.lseq t (U32.v (length a))))
@@ -173,7 +180,8 @@ val glue_array
   : m_action
     (star (pts_to_array a p iseq) (pts_to_array a' p iseq'))
     (new_a:array_ref t{
-      address new_a = address a /\ max_length new_a = max_length a /\
+      (a =!= null_array t ==> (new_a =!= null_array t /\ address new_a = address a)) /\
+      max_length new_a = max_length a /\
       offset new_a = offset a /\ length new_a = U32.add (length a) (length a')
     })
     (fun new_a -> pts_to_array new_a p (Seq.Base.append iseq iseq'))
